...

theories/Closure.v
@@ -1,7 +1,7 @@
 Require Import Unicode.Utf8.
 Require Import Coq.Program.Equality.
 Require Import Coq.Logic.FunctionalExtensionality.
-
+Require Import Coq.omega.Omega.
 From mathcomp Require Import ssreflect.
 
 From gctt Require Import OrderTheory.
@@ -10,6 +10,7 @@ From gctt Require Import Axioms.
 From gctt Require Import Terms.
 
 
+Set Bullet Behavior "Strict Subproofs".
 
 From gctt Require Tactic.
 Module T := Tactic.
@@ -176,8 +177,8 @@ Module Clo.
     try by [contradiction];
     rewrite /M.empty;
     move=> *; simpl in *;
-    T.destruct_conjs;
-    T.destruct_evals.
+    T.destruct_conjs.
+
 
 
   Ltac destruct_clo :=
@@ -198,11 +199,145 @@ Module Clo.
       | H : ∀ R1 R2 : M.behavior, t _ (?X, _) → t _ (?X, _) → _ = _, H' : t _ (?X, ?R1), H'' : t _ (?X, ?R2) |- _ => specialize (H _ _ H' H''); move: H
   end.
 
+  Inductive type_value_candidate : Tm.val 0 → Prop :=
+  | unit : type_value_candidate Tm.unit
+  | bool : type_value_candidate Tm.bool
+  | prod : ∀ A B, type_value_candidate (Tm.prod A B)
+  | ltr : ∀ κ A, type_value_candidate (Tm.ltr κ A)
+  | isect : ∀ A, type_value_candidate (Tm.isect A)
+  | univ : ∀ i, type_value_candidate (Tm.univ i).
+  Hint Constructors type_value_candidate.
+
+  Theorem value_of_type : ∀ A R, t M.empty (A, R) → ∃ A0, A ⇓ A0 ∧ type_value_candidate A0 ∧ t M.empty (Tm.ret A0, R).
+  Proof.
+    move=> A R T.
+    apply: (ind T) => //= T'; T.destruct_conjs.
+    + repeat T.split; eauto.
+      rewrite -roll.
+      apply: Sig.unit.
+      split; auto.
+    + repeat T.split; eauto.
+      rewrite -roll; apply: Sig.bool.
+      split; auto.
+    + repeat T.split; eauto.
+      rewrite -roll; apply: Sig.prod.
+      repeat T.split; eauto.
+    + repeat T.split; eauto.
+      rewrite -roll; apply: Sig.isect.
+      repeat T.split; eauto.
+    + repeat T.split; eauto.
+      rewrite -roll; apply: Sig.later.
+      repeat T.split; eauto.
+  Qed.
+
+
+  Axiom determinacy : ∀ A A0 A1, A ⇓ A0 → A ⇓ A1 → A0 = A1.
+
+  Ltac eval_destruction :=
+    match goal with | H : _ ⇓ _ |- _ => dependent destruction H end.
+
+
+  Ltac by_eval_inversion :=
+    match goal with | H : _ ⇓ _ |- _ => by [inversion H] end.
+
+
+  Ltac invert_type_val :=
+    match goal with
+    | H : type_value_candidate _ |- _ => dependent destruction H
+    | H1 : ?A ⇓ ?A0, H2 : ?A ⇓ ?A1, H3 : ?A0 = ?A1 |- _ => idtac
+    | H1 : ?A ⇓ ?A0, H2 : ?A ⇓ ?A0 |- _ => clear H2
+    | H1 : ?A ⇓ ?A0, H2 : ?A ⇓ ?A1 |- _ =>
+      let x := fresh in have x: A0 = A1; [by [apply: determinacy H1 H2] | try discriminate]
+    end.
+
+
+
 
   Theorem functionality : M.functional (t M.empty).
   Proof.
+    move=> A R1 R2.
+    move=> T1; case: (value_of_type T1) => {T1} A01 [eval1 [cand1 T1]].
+    move=> T2; case: (value_of_type T2) => {T2} A02 [eval2 [cand2 T2]].
+    move: A01 A02 cand1 cand2 eval1 eval2 T1 T2.
+    repeat invert_type_val.
+    + admit.
+    + admit.
+    + rewrite H in T1.
+      destruct_clos => //= *; T.destruct_conjs;
+      repeat invert_type_val; try by_eval_inversion.
+      eval_destruction.
+      T.destruct_evals.
+      repeat eval_inversion..
+
+    + invert_type_val.
+    + invert_type_val.
+    + invert_type_val.
+
+
+
+    + admit.
+    + admit.
+    +
+    invert_type_val.
+    invert_type_val.
+    invert_type_val.
+    admit.
+    repeat invert_type_val.
+    discriminate.
+
+
+
+
+    repeat invert_type_val.
+    repeat invert_type_val.
+    move: A01 A02 A eval1 eval2 R1 R2 T1 T2.
+    elim.
+    + move=> A02 A cand1 cand2 eval1 eval2 //= *.
+
+
+      repeat invert_type_val.
+      move=> *.
+
+      case: (determinacy eval1 eval2) => p.
+      rewrite -p.
+      move=> R1 R2 T1 T2.
+      destruct_clos => //= *; T.destruct_conjs; try by [eval_inversion].
+      congruence.
+    + admit.
+    + admit.
+    + admit.
+    + admit.
+    + admit.
+    + admit.
+    + admit.
+    + admit.
+    + admit.
+    + admit.
+
+      repeat match goal with | H : _ ⇓ _ |- _ => dependent destruction H end.
+
+
+      ++ congruence.
+      ++ eval_inversion.
+
+
+
+    + admit.
+    + admit.
+    + admit.
+    + admit.
+
+    dependent induction eval1; dependent induction eval2.
+
+    + move=> *; destruct_clos => //= *.
+      noconfusion.
+
+
+
+    apply: (value_of_type T).
+
     elim; rewrite /M.based_functional;
-    move=> *; try by [destruct_clos => //= *; noconfusion];
+    move=> *; try by [destruct_clos => //= *; noconfusion].
     destruct_clos => *; noconfusion.
     + congruence.
     + congruence.
